@prefix dc: <http://purl.org/dc/elements/1.1/> .
@prefix dcterms: <http://purl.org/dc/terms/> .
@prefix owl: <http://www.w3.org/2002/07/owl#> .
@prefix rdf: <http://www.w3.org/1999/02/22-rdf-syntax-ns#> .
@prefix rdfs: <http://www.w3.org/2000/01/rdf-schema#> .
@prefix sh: <http://www.w3.org/ns/shacl#> .
@prefix xisadg: <https://github.com/KOST-CECO/ontologies/blob/master/xisadg#> .
@prefix xsd: <http://www.w3.org/2001/XMLSchema#> .

<https://github.com/KOST-CECO/ontologies/blob/master/xisadg>
  rdf:type owl:Ontology ;
  owl:imports <http://datashapes.org/dash> ;
  owl:imports dc: ;
  owl:imports dcterms: ;
  owl:versionInfo "Created with TopBraid Composer" ;
.

xisadg:ArchivalDescription
  rdf:type rdfs:Class ;
  rdf:type sh:NodeShape ;
  rdfs:comment "Globales Element für die Beschreibung einer Verzeichnungseinheit"@de ;
  rdfs:comment "global element for an ISADG-description of an description unit"@en ;
  rdfs:comment "élement globale pour la description d'une unité de description"@fr ;
  rdfs:subClassOf rdfs:Resource ;
.

xisadg:hasArchivalDescription
  rdf:type owl:IrreflexiveProperty ;
  rdf:type owl:TransitiveProperty ;
  rdfs:domain "xisadg:ArchivalDescription"^^rdfs:Class ;
  rdfs:range "xisadg:ArchivalDescription"^^rdfs:Class ;
  rdfs:subPropertyOf dcterms:hasPart ;
.

xisadg:hasContext
  rdf:type rdf:Property ;
  rdfs:comment "Area delle informazioni sul contesto"@it ;
  rdfs:comment "Kontext"@de ;
  rdfs:comment "Zone du contexte"@fr ;
  rdfs:comment "context area"@en ;
  rdfs:label "2 context" ;
.

xisadg:hasIdentity
  rdf:type rdf:Property ;
  rdfs:comment "Area dell'identificazione"@it ;
  rdfs:comment "Identifikation"@de ;
  rdfs:comment "Zone d'identification"@fr ;
  rdfs:comment "identity statement area"@en ;
  rdfs:label "1 identity" ;
  rdfs:subPropertyOf xisadg:hasStatement ;
.
